more examples for tutorial

pulse/share/steel/examples/pulse/by-example/PulseTutorial.ImplicationAndForall.fst
@@ -1,304 +1,131 @@
 module PulseTutorial.ImplicationAndForall
 open Pulse.Lib.Pervasives
-module S = Pulse.Lib.Stick.Util
-module FA = Pulse.Lib.Forall.Util
-open FStar.List.Tot
-
-//llist$
-noeq
-type node (t:Type0) = {
-    head : t;
-    tail : llist t;
-}
-
-and node_ptr (t:Type0) = ref (node t)
-
-//A nullable pointer to a node
-and llist (t:Type0) = option (node_ptr t)
-//llist$
-
-//is_list$
-let rec is_list #t (x:llist t) (l:list t)
-: Tot vprop (decreases l)
-= match l with
-  | [] -> pure (x == None)
-  | head::tl -> 
-    exists* (p:node_ptr t) (tail:llist t).
-      pure (x == Some p) **
-      pts_to p { head; tail } **
-      is_list tail tl
-//is_list$
-
-//boilerplate$
-```pulse
-ghost
-fn elim_is_list_nil (#t:Type0) (x:llist t)
-requires is_list x l ** pure (l == [])
-ensures pure (x == None)
-{
-   rewrite each l as Nil #t;
-   unfold (is_list x [])
-}
-```
-
-```pulse
-ghost
-fn intro_is_list_nil (#t:Type0) (x:llist t)
-requires pure (x == None)
-ensures is_list x []
-{
-    fold (is_list x []);
-}
-```
-
-```pulse
-ghost
-fn elim_is_list_cons (#t:Type0) (x:llist t) (l:list t) (head:t) (tl:list t)
-requires is_list x l ** pure (l == head::tl)
-ensures (
-  exists* (p:node_ptr t) (tail:llist t).
-    pure (x == Some p) **
-    pts_to p { head; tail } **
-    is_list tail tl
-)
-{
-  rewrite each l as (head::tl);
-  rewrite_by
-    (is_list x (head::tl))
-    (exists* (p:node_ptr t) (tail:llist t).
-      pure (x == Some p) **
-      pts_to p { head; tail } **
-      is_list tail tl)
-    vprop_equiv_norm
-    ()
-}
-```
-    
-
-```pulse
-ghost
-fn intro_is_list_cons (#t:Type0) (x:llist t) (v:node_ptr t) (#node:node t) (#tl:list t)
-requires
-  pts_to v node **
-  is_list node.tail tl **
-  pure (x == Some v)
-ensures
-  is_list x (node.head::tl)
-{
-    rewrite (pts_to v node) as (pts_to v { head=node.head; tail=node.tail });
-    rewrite_by
-        (exists* (v:node_ptr t) (tail:llist t).
-          pure (x == Some v) **
-          pts_to v { head=node.head; tail } **
-          is_list tail tl)
-        (is_list x (node.head::tl))
-        vprop_equiv_norm
-        ()
-}
-```
-//boilerplate$
-
-//is_list_cases$
-let is_list_cases #t (x:llist t) (l:list t)
-: vprop 
-= match x with
-  | None -> pure (l == [])
-  | Some v -> 
-    exists* (n:node t) (tl:list t).
-      pts_to v n **
-      pure (l == n.head::tl) **
-      is_list n.tail tl
-//is_list_cases$
-
-```pulse //cases_of_is_list$
-ghost
-fn cases_of_is_list #t (x:llist t) (l:list t)
-requires is_list x l
-ensures is_list_cases x l
-{
-  match l {
-    Nil -> { 
-      elim_is_list_nil x;
-      fold (is_list_cases None l);
-      rewrite each (None #(ref (node t))) as x;
-    }
-    Cons head tl -> { 
-      elim_is_list_cons x l head tl;
-      with w tail. _;
-      let v = Some?.v x;
-      rewrite each w as v;
-      rewrite each tail as (({ head; tail }).tail) in (is_list tail tl);
-      fold (is_list_cases (Some v) l);
-      rewrite each (Some #(ref (node t)) v) as x;
-    }
-  }
-}
-```
-
-```pulse //is_list_case_none$
-ghost
-fn is_list_case_none (#t:Type) (x:llist t) (#l:list t)
-requires is_list x l ** pure (x == None)
-ensures is_list x l ** pure (l == [])
-{
-  cases_of_is_list x l;
-  rewrite each x as (None #(ref (node t)));
-  unfold (is_list_cases None l);
-  intro_is_list_nil x;
-}
-```
-
-
-```pulse //is_list_case_some$
-ghost
-fn is_list_case_some (#t:Type) (x:llist t) (v:node_ptr t) (#l:list t) 
-requires is_list x l ** pure (x == Some v)
-ensures
-  exists* (node:node t) (tl:list t).
-    pts_to v node **
-    is_list node.tail tl **
-    pure (l == node.head::tl)
-{
-  cases_of_is_list x l;
-  rewrite each x as (Some v);
-  unfold (is_list_cases (Some v) l);
-}
-```
-
-
-```pulse //length$
-fn rec length (#t:Type0) (x:llist t)
-requires is_list x 'l
-returns n:nat
-ensures is_list x 'l ** pure (n == List.Tot.length 'l)
-{
-  match x {
-    None -> {
-      is_list_case_none x;
-      0
-    }
-    Some vl -> {
-      is_list_case_some x vl;
-      with _node _tl. _;
-      let node = !vl;
-      rewrite each _node.tail as node.tail; 
-      let n = length #t node.tail;
-      intro_is_list_cons x vl;
-      (1 + n)
-    }
-  }
-}
-```
-
-```pulse
-fn rec length_tail (#t:Type0) (x:llist t) (k:nat)
-requires is_list x 'l
-returns n:nat
-ensures is_list x 'l ** pure (n == k + List.Tot.length 'l)
-{
-  match x {
-    None -> {
-      is_list_case_none x;
-      k
-    }
-    Some vl -> {
-      is_list_case_some x vl;
-      with tail tl. assert (is_list #t tail tl);
-      let n = !vl;
-      rewrite each tail as n.tail; 
-      let n = length_tail #t n.tail (1 + k);
-      intro_is_list_cons x vl;
-      n
-    }
-  }
-}
-```
-
+open Pulse.Lib.Stick.Util
+open Pulse.Lib.Forall.Util
 module I = Pulse.Lib.Stick.Util
-open I
+module GR = Pulse.Lib.GhostReference
+open GR
 
-```pulse
-ghost
-fn list_cons_if_list_tail (#t:Type) 
-                          (v:node_ptr t)
-                          (tl:erased (list t))
-requires 
-  pts_to v n
-ensures 
-  (is_list n.tail tl @==> is_list (Some v) (n.head::tl))
+//regain_half$
+let regain_half #a (x:GR.ref a) (v:a) =
+  pts_to x #one_half v @==> pts_to x v
+//regain_half$
+
+
+```pulse //intro_regain_half$
+ghost 
+fn intro_regain_half (x:GR.ref int)
+requires pts_to x 'v
+ensures pts_to x #one_half 'v ** regain_half x 'v
 {
   ghost
-  fn yields_elim ()
-  requires 
-    pts_to v n ** is_list n.tail tl
-  ensures 
-    is_list (Some v) (n.head::tl)
+  fn aux ()
+  requires pts_to x #one_half 'v ** pts_to x #one_half 'v
+  ensures pts_to x 'v
   {
-    intro_is_list_cons (Some v) v
+    GR.gather x;
   };
-  I.intro _ _ _ yields_elim;
+  GR.share x;
+  I.intro _ _ _ aux;
+  fold regain_half;
 }
 ```
 
-
-```pulse
-fn move_next (#t:Type) (x:llist t)
-    requires is_list x 'l ** pure (Some? x)
-    returns y:llist t
-    ensures exists* tl.
-        is_list y tl **
-        (is_list y tl @==> is_list x 'l) **
-        pure (Cons? 'l /\ tl == Cons?.tl 'l)
-{ 
-    let np = Some?.v x;
-    is_list_case_some x np;
-    let node = !np;
-    with tail tl. assert (is_list #t tail tl);
-    rewrite each tail as node.tail;
-    list_cons_if_list_tail np tl;
-    node.tail
-}
-```
-
-```pulse
-fn length_iter (#t:Type) (x: llist t)
-    requires is_list x 'l
-    returns n:nat
-    ensures is_list x 'l ** pure (n == List.Tot.length 'l)
+```pulse //use_regain_half$
+ghost
+fn use_regain_half (x:GR.ref int)
+requires pts_to x #one_half 'v ** regain_half x 'v
+ensures pts_to x 'v
 {
-  open I;
-  let mut cur = x;
-  let mut ctr = 0; 
-  I.refl (is_list x 'l);
-  while (
-    with _b _n ll _sfx. _; 
-    let v = !cur; 
-    rewrite (pts_to cur v) as (pts_to cur ll);
-    Some? v
-  )
-  invariant b.  
-  exists* n ll suffix.
-    pts_to ctr n **
-    pts_to cur ll **
-    is_list ll suffix **
-    (is_list ll suffix @==> is_list x 'l) **
-    pure (n == List.Tot.length 'l - List.Tot.length suffix) **
-    pure (b == (Some? ll))
-  {
-    with _n _ll suffix. _;
-    let n = !ctr;
-    let ll = !cur;
-    rewrite each _ll as ll;
-    let next = move_next ll;
-    with tl. assert (is_list next tl);
-    I.trans (is_list next tl) (is_list ll suffix) (is_list x 'l);
-    cur := next;
-    ctr := n + 1;
-  };
-  with _n ll _sfx. _;
-  is_list_cases_none ll;
+  unfold regain_half;
   I.elim _ _;
-  let n = !ctr;
-  n
 }
 ```
+
+//regain_half_q$
+let regain_half_q #a (x:GR.ref a) =
+  forall* u. pts_to x #one_half u @==> pts_to x u 
+//regain_half_q$
+
+
+module FA = Pulse.Lib.Forall.Util
+
+```pulse //intro_regain_half_q$
+ghost 
+fn intro_regain_half_q (x:GR.ref int)
+requires pts_to x 'v
+ensures pts_to x #one_half 'v ** regain_half_q x
+{
+  ghost
+  fn aux1 (u:int)
+  requires pts_to x #one_half 'v ** pts_to x #one_half u
+  ensures pts_to x u
+  {
+    gather x;
+  };
+  GR.share x;
+  FA.intro_forall_imp _ _ _ aux1;
+  fold regain_half_q;
+}
+```
+
+```pulse //use_regain_half_q$
+ghost
+fn use_regain_half_q (x:GR.ref int)
+requires pts_to x #one_half 'u ** regain_half_q x
+ensures pts_to x 'u
+{
+  unfold regain_half_q;
+  FA.elim #_ #(fun u -> pts_to x #one_half u @==> pts_to x u) 'u;
+  I.elim _ _;
+}
+```
+
+//can_update$
+let can_update (x:GR.ref int) = 
+  forall* u v. pts_to x #one_half u @==>
+               pts_to x v
+//can_update$
+
+```pulse //make_can_update$
+ghost
+fn make_can_update (x:GR.ref int)
+requires pts_to x w
+ensures pts_to x #one_half w ** can_update x
+{
+  ghost
+  fn aux (u:int)
+  requires pts_to x #one_half w
+  ensures forall* v. pts_to x #one_half u @==> pts_to x v
+  {
+    ghost
+    fn aux (v:int)
+    requires pts_to x #one_half w ** pts_to x #one_half u
+    ensures pts_to x v
+    {
+      gather x;
+      x := v;
+    };
+    FA.intro_forall_imp _ _ _ aux;
+  };
+  share x;
+  FA.intro _ aux;
+  fold (can_update x);
+}
+```
+
+```pulse //update$
+ghost
+fn update (x:GR.ref int) (k:int)
+requires pts_to x #one_half 'u ** can_update x
+ensures pts_to x #one_half k ** can_update x
+{
+  unfold can_update;
+  FA.elim #_ #(fun u -> forall* v. pts_to x #one_half u @==> pts_to x v) 'u;
+  FA.elim #_ #(fun v -> pts_to x #one_half 'u @==> pts_to x v) k;
+  I.elim _ _;
+  make_can_update x;
+}
+```
+
+
