pulse/share/steel/examples/pulse/by-example/PulseTutorial.LinkedList.fst
@@ -1,0 +1,310 @@
+module PulseTutorial.LinkedList
+open Pulse.Lib.Pervasives
+module S = Pulse.Lib.Stick.Util
+module FA = Pulse.Lib.Forall.Util
+open FStar.List.Tot
+
+//llist$
+noeq
+type node (t:Type0) = {
+    head : t;
+    tail : llist t;
+}
+
+and node_ptr (t:Type0) = ref (node t)
+
+//A nullable pointer to a node
+and llist (t:Type0) = option (node_ptr t)
+//llist$
+
+//is_list$
+let rec is_list #t (x:llist t) (l:list t)
+: Tot vprop (decreases l)
+= match l with
+  | [] -> pure (x == None)
+  | head::tl -> 
+    exists* (p:node_ptr t) (tail:llist t).
+      pure (x == Some p) **
+      pts_to p { head; tail } **
+      is_list tail tl
+//is_list$
+
+//boilerplate$
+```pulse
+ghost
+fn elim_is_list_nil (#t:Type0) (x:llist t)
+requires is_list x l ** pure (l == [])
+ensures pure (x == None)
+{
+   rewrite each l as Nil #t;
+   unfold (is_list x [])
+}
+```
+
+```pulse
+ghost
+fn intro_is_list_nil (#t:Type0) (x:llist t)
+requires pure (x == None)
+ensures is_list x []
+{
+    fold (is_list x []);
+}
+```
+
+```pulse
+ghost
+fn elim_is_list_cons (#t:Type0) (x:llist t) (l:list t) (head:t) (tl:list t)
+requires is_list x l ** pure (l == head::tl)
+ensures (
+  exists* (p:node_ptr t) (tail:llist t).
+    pure (x == Some p) **
+    pts_to p { head; tail } **
+    is_list tail tl
+)
+{
+  rewrite each l as (head::tl);
+  rewrite_by
+    (is_list x (head::tl))
+    (exists* (p:node_ptr t) (tail:llist t).
+      pure (x == Some p) **
+      pts_to p { head; tail } **
+      is_list tail tl)
+    vprop_equiv_norm
+    ()
+}
+```
+    
+
+```pulse
+ghost
+fn intro_is_list_cons (#t:Type0) (x:llist t) (v:node_ptr t) (#node:node t) (#tl:list t)
+requires
+  pts_to v node **
+  is_list node.tail tl **
+  pure (x == Some v)
+ensures
+  is_list x (node.head::tl)
+{
+    rewrite (pts_to v node) as (pts_to v { head=node.head; tail=node.tail });
+    rewrite_by
+        (exists* (v:node_ptr t) (tail:llist t).
+          pure (x == Some v) **
+          pts_to v { head=node.head; tail } **
+          is_list tail tl)
+        (is_list x (node.head::tl))
+        vprop_equiv_norm
+        ()
+}
+```
+//boilerplate$
+
+//is_list_cases$
+let is_list_cases #t (x:llist t) (l:list t)
+: vprop 
+= match x with
+  | None -> pure (l == [])
+  | Some v -> 
+    exists* (n:node t) (tl:list t).
+      pts_to v n **
+      pure (l == n.head::tl) **
+      is_list n.tail tl
+//is_list_cases$
+
+```pulse //cases_of_is_list$
+ghost
+fn cases_of_is_list #t (x:llist t) (l:list t)
+requires is_list x l
+ensures is_list_cases x l
+{
+  match l {
+    Nil -> { 
+      elim_is_list_nil x;
+      fold (is_list_cases None l);
+      rewrite each (None #(ref (node t))) as x;
+    }
+    Cons head tl -> { 
+      elim_is_list_cons x l head tl;
+      with w tail. _;
+      let v = Some?.v x;
+      rewrite each w as v;
+      rewrite each tail as (({ head; tail }).tail) in (is_list tail tl);
+      fold (is_list_cases (Some v) l);
+      rewrite each (Some #(ref (node t)) v) as x;
+    }
+  }
+}
+```
+
+```pulse //is_list_case_none$
+ghost
+fn is_list_case_none (#t:Type) (x:llist t) (#l:list t)
+requires is_list x l ** pure (x == None)
+ensures is_list x l ** pure (l == [])
+{
+  cases_of_is_list x l;
+  rewrite each x as (None #(ref (node t)));
+  unfold (is_list_cases None l);
+  intro_is_list_nil x;
+}
+```
+
+
+```pulse //is_list_case_some$
+ghost
+fn is_list_case_some (#t:Type) (x:llist t) (v:node_ptr t) (#l:list t) 
+requires is_list x l ** pure (x == Some v)
+ensures
+  exists* (node:node t) (tl:list t).
+    pts_to v node **
+    is_list node.tail tl **
+    pure (l == node.head::tl)
+{
+  cases_of_is_list x l;
+  rewrite each x as (Some v);
+  unfold (is_list_cases (Some v) l);
+}
+```
+
+
+```pulse //length$
+fn rec length (#t:Type0) (x:llist t)
+requires is_list x 'l
+returns n:nat
+ensures is_list x 'l ** pure (n == List.Tot.length 'l)
+{
+  match x {
+    None -> {
+      is_list_case_none x;
+      0
+    }
+    Some vl -> {
+      is_list_case_some x vl;
+      with _node _tl. _;
+      let node = !vl;
+      rewrite each _node.tail as node.tail; 
+      let n = length #t node.tail;
+      intro_is_list_cons x vl;
+      (1 + n)
+    }
+  }
+}
+```
+
+```pulse
+fn rec length_tail (#t:Type0) (x:llist t) (k:nat)
+requires is_list x 'l
+returns n:nat
+ensures is_list x 'l ** pure (n == k + List.Tot.length 'l)
+{
+  match x {
+    None -> {
+      is_list_case_none x;
+      k
+    }
+    Some vl -> {
+      is_list_case_some x vl;
+      with tail tl. assert (is_list #t tail tl);
+      let n = !vl;
+      rewrite each tail as n.tail; 
+      let n = length_tail #t n.tail (1 + k);
+      intro_is_list_cons x vl;
+      n
+    }
+  }
+}
+```
+
+module I = Pulse.Lib.Stick.Util
+open I
+
+```pulse
+ghost
+fn list_cons_if_list_tail (#t:Type) 
+                          (v:node_ptr t)
+                          (tl:erased (list t))
+requires 
+  pts_to v n
+ensures 
+  (is_list n.tail tl @==> is_list (Some v) (n.head::tl))
+{
+  ghost
+  fn yields_elim ()
+  requires 
+    pts_to v n ** is_list n.tail tl
+  ensures 
+    is_list (Some v) (n.head::tl)
+  {
+    intro_is_list_cons (Some v) v
+  };
+  I.intro _ _ _ yields_elim;
+}
+```
+
+
+```pulse
+fn move_next (#t:Type) (x:llist t)
+    requires is_list x 'l ** pure (Some? x)
+    returns y:llist t
+    ensures exists* tl.
+        is_list y tl **
+        (is_list y tl @==> is_list x 'l) **
+        pure (Cons? 'l /\ tl == Cons?.tl 'l)
+{ 
+    let np = Some?.v x;
+    is_list_case_some x np;
+    let node = !np;
+    with tail tl. assert (is_list #t tail tl);
+    rewrite each tail as node.tail;
+    list_cons_if_list_tail np tl;
+    node.tail
+}
+```
+
+module GR = Pulse.Lib.GhostReference
+open Pulse.Lib.Forall.Util
+let can_update (x:GR.ref int) = 
+  forall* v. pts_to x #half_perm v @==>
+             pts_to x #half_perm (v + 1)
+
+```pulse
+fn length_iter (#t:Type) (x: llist t)
+    requires is_list x 'l
+    returns n:nat
+    ensures is_list x 'l ** pure (n == List.Tot.length 'l)
+{
+  open I;
+  let mut cur = x;
+  let mut ctr = 0; 
+  I.refl (is_list x 'l);
+  while (
+    with _b _n ll _sfx. _; 
+    let v = !cur; 
+    rewrite (pts_to cur v) as (pts_to cur ll);
+    Some? v
+  )
+  invariant b.  
+  exists* n ll suffix.
+    pts_to ctr n **
+    pts_to cur ll **
+    is_list ll suffix **
+    (is_list ll suffix @==> is_list x 'l) **
+    pure (n == List.Tot.length 'l - List.Tot.length suffix) **
+    pure (b == (Some? ll))
+  {
+    with _n _ll suffix. _;
+    let n = !ctr;
+    let ll = !cur;
+    rewrite each _ll as ll;
+    let next = move_next ll;
+    with tl. assert (is_list next tl);
+    I.trans (is_list next tl) (is_list ll suffix) (is_list x 'l);
+    cur := next;
+    ctr := n + 1;
+  };
+  with _n ll _sfx. _;
+  is_list_cases_none ll;
+  I.elim _ _;
+  let n = !ctr;
+  n
+}
+```
